Rename the DFSM from slide 16
Now naming it as it appears in the textbook, as "Example 5.4", rather
than based on on the slide number in the presentation of Chapter 5,
in preparation for my Dafny 2026 talk.

Also renumber the states to avoid unneeded confusion.

simulators/FSM_Simulators-py/FSM__SIMULATION.py
@@ -112,7 +112,7 @@ class default__:
         return accepted
 
     @staticmethod
-    def delta__16(k, c):
+    def delta__5__4(k, c):
         if ((k) == (default__.q0)) and ((c) == (_dafny.CodePoint('0'))):
             return default__.q0
         elif ((k) == (default__.q0)) and ((c) == (_dafny.CodePoint('1'))):
@@ -126,10 +126,10 @@ class default__:
     def Main(noArgsParameter__):
         d_0_accepted_: bool
         out0_: bool
-        out0_ = default__.dfsmsimulate(default__.M__16, _dafny.SeqWithoutIsStrInference(map(_dafny.CodePoint, "1001")))
+        out0_ = default__.dfsmsimulate(default__.M__5__4, _dafny.SeqWithoutIsStrInference(map(_dafny.CodePoint, "1001")))
         d_0_accepted_ = out0_
         out1_: bool
-        out1_ = default__.dfsmsimulate(default__.M__16, _dafny.SeqWithoutIsStrInference(map(_dafny.CodePoint, "10011")))
+        out1_ = default__.dfsmsimulate(default__.M__5__4, _dafny.SeqWithoutIsStrInference(map(_dafny.CodePoint, "10011")))
         d_0_accepted_ = out1_
         out2_: bool
         out2_ = default__.ndfsmsimulate(default__.M__59, _dafny.SeqWithoutIsStrInference(map(_dafny.CodePoint, "")))
@@ -145,26 +145,26 @@ class default__:
         d_0_accepted_ = out5_
 
     @_dafny.classproperty
-    def K__16(instance):
-        return _dafny.Set({5, 8})
+    def K__5__4(instance):
+        return _dafny.Set({0, 1})
     @_dafny.classproperty
-    def Sigma__16(instance):
+    def Sigma__5__4(instance):
         return _dafny.Set({_dafny.CodePoint('0'), _dafny.CodePoint('1')})
     @_dafny.classproperty
     def q0(instance):
-        return 5
+        return 0
     @_dafny.classproperty
     def q1(instance):
-        return 8
+        return 1
     @_dafny.classproperty
-    def s__16(instance):
+    def s__5__4(instance):
         return default__.q0
     @_dafny.classproperty
-    def A__16(instance):
+    def A__5__4(instance):
         return _dafny.Set({default__.q1})
     @_dafny.classproperty
-    def M__16(instance):
-        return (default__.K__16, default__.Sigma__16, default__.delta__16, default__.s__16, default__.A__16)
+    def M__5__4(instance):
+        return (default__.K__5__4, default__.Sigma__5__4, default__.delta__5__4, default__.s__5__4, default__.A__5__4)
     @_dafny.classproperty
     def K__59(instance):
         return _dafny.Set({0, 1, 2, 3, 4, 5, 6})
